Complete sheets 3-3 and 3-4

src/section03groups/sheet4.lean
@@ -55,17 +55,20 @@ variable (f : G →** H)
 -- is called. Uncomment it, look at the output, and remember it. It's
 -- a useful part of the group theory API.
 
--- example (a b : G) : a * b = b ↔ a = 1 := by library_search -- look at the output.
+example (a b : G) : a * b = b ↔ a = 1 := mul_left_eq_self
 
 -- Now see if you can do these.
 @[simp] lemma map_one : f 1 = 1 :=
 begin
-  sorry
+  have h : f 1 * f 1 = f (1 * 1) := (map_mul f 1 1).symm,
+  simpa using h,
 end
 
 lemma map_inv (a : G) : f a⁻¹ = (f a)⁻¹ :=
 begin
-  sorry,
+  have h : f a * f a⁻¹ = f (a * a⁻¹) := (map_mul f a a⁻¹).symm,
+  simp at h,
+  exact (mul_eq_one_iff_inv_eq.mp h).symm,
 end
 
 variable (G)
@@ -73,14 +76,18 @@ variable (G)
 /-- `id G` is the identity group homomorphism from `G` to `G`. -/
 def id : G →** G :=
 { to_fun := λ a, a,
-  map_mul' := begin sorry end } -- fill in the proof that the identity function is a group hom!
+  map_mul' := begin simp, end } -- fill in the proof that the identity function is a group hom!
 
 variables {K : Type} [group K] {G}
 
 /-- `φ.comp ψ` is the composite of `φ` and `ψ`. -/
 def comp (φ : G →** H) (ψ : H →** K) : G →** K :=
 { to_fun := λ g, ψ (φ g),
-  map_mul' := begin sorry end -- fill in the proof that composite of two group homs is a group hom!
+  map_mul' :=
+  begin
+    simp_rw [map_mul φ, ← map_mul ψ],
+    simp,
+  end -- fill in the proof that composite of two group homs is a group hom!
 }
 
 -- The next three lemmas are pretty standard, but they are also in fact
@@ -90,50 +97,108 @@ def comp (φ : G →** H) (ψ : H →** K) : G →** K :=
 -- with the `ext` tactic.
 lemma id_comp : (id G).comp f = f :=
 begin
-  sorry
+  ext,
+  refl,
 end
 
 lemma comp_id : f.comp (id H) = f :=
 begin
-  sorry
+  ext,
+  refl,
 end
 
 lemma comp_assoc {L : Type} [group L] (φ : G →** H) (ψ : H →** K) (ρ : K →** L) :
   (φ.comp ψ).comp ρ = φ.comp (ψ.comp ρ) :=
 begin
-  sorry,
+  refl,
 end
 
 /-- The kernel of a group homomorphism, as a subgroup of the source group. -/
 def ker (f : G →** H) : subgroup G :=
 { carrier := {g : G | f g = 1 },
-  one_mem' := begin sorry end,
-  mul_mem' := begin sorry end,
-  inv_mem' := begin sorry end,
+  one_mem' := f.map_one,
+  mul_mem' := begin
+    intros a b ha hb,
+    change f a = 1 at ha,
+    change f b = 1 at hb,
+    change f (a * b) = 1,
+    rw [f.map_mul, ha, hb, one_mul],
+  end,
+  inv_mem' := begin
+    intros x hx,
+    simp [map_inv, *] at *,
+  end,
 }
 
 /-- The image of a group homomorphism, as a subgroup of the target group. -/
 def im (f : G →** H) : subgroup H :=
 { carrier := {h : H | ∃ g : G, f g = h },
-  one_mem' := begin sorry end,
-  mul_mem' := begin sorry end,
-  inv_mem' := begin sorry end,
+  one_mem' := begin
+    use 1,
+    simp,
+  end,
+  mul_mem' := begin
+    intros a b ha hb,
+    simp at *,
+    cases ha with x ha,
+    cases hb with y hb,
+    use x * y,
+    simp [f.map_mul, *],
+  end,
+  inv_mem' := begin
+    intros x hx,
+    simp at *,
+    cases hx with y hx,
+    use y⁻¹,
+    simp [f.map_inv, *],
+  end,
 }
 
 /-- The image of a subgroup under a group homomorphism, as a subgroup. -/
 def map (f : G →** H) (K : subgroup G) : subgroup H :=
 { carrier := {h : H | ∃ g : G, g ∈ K ∧ f g = h },
-  one_mem' := begin sorry end,
-  mul_mem' := begin sorry end,
-  inv_mem' := begin sorry end,
+  one_mem' := begin
+    simp,
+    use 1,
+    exact ⟨K.one_mem, f.map_one⟩,
+  end,
+  mul_mem' := begin
+    intros a b ha hb,
+    simp at *,
+    rcases ha with ⟨x, hx1, hx2⟩,
+    rcases hb with ⟨y, hy1, hy2⟩,
+    use x * y,
+    split,
+    { exact K.mul_mem hx1 hy1 },
+    { rw [f.map_mul, hx2, hy2] }
+  end,
+  inv_mem' := begin
+    intros x hx,
+    simp at *,
+    rcases hx with ⟨y, hy1, hy2⟩,
+    use y⁻¹,
+    split,
+    { exact K.inv_mem hy1 },
+    { rw [f.map_inv, hy2] }
+  end,
 }
 
 /-- The preimage of a subgroup under a group homomorphism, as a subgroup. -/
 def comap (f : G →** H) (K : subgroup H) : subgroup G :=
 { carrier := {g : G | f g ∈ K },
-  one_mem' := begin sorry end,
-  mul_mem' := begin sorry end,
-  inv_mem' := begin sorry end,
+  one_mem' := begin
+    simpa using K.one_mem,
+  end,
+  mul_mem' := begin
+    simp [f.map_mul],
+    intros a b ha hb,
+    exact K.mul_mem ha hb,
+  end,
+  inv_mem' := begin
+    simp,
+    intros x hx,
+    simpa [f.map_inv] using K.inv_mem hx,
+  end,
 }
 
 /-- Pushing a subgroup along one homomorphism and then another is equal to
@@ -141,7 +206,9 @@ def comap (f : G →** H) (K : subgroup H) : subgroup G :=
 lemma map_comp (φ : G →** H) (ψ : H →** K) (L : subgroup G) :
   (φ.comp ψ).map L = ψ.map (φ.map L) :=
 begin
-  sorry
+  ext,
+  simp [map, map],
+  split; intro h; exact h,
 end
 
 /-- Pulling a subgroup back along one homomorphism and then another, is equal
@@ -149,7 +216,9 @@ to pulling it back along the composite of the homomorphisms. -/
 lemma comap_comp (φ : G →** H) (ψ : H →** K) (L : subgroup K) :
   (φ.comp ψ).comap L = φ.comap (ψ.comap L) :=
 begin
-  sorry
+  ext,
+  simp [comap, comap],
+  split; intro h; exact h
 end
 
 end my_group_hom
